Simplify conditions on CSE analysis result.
If we know that the value numbers are equal we can simplify some integer
comparisons since we then know that they either always evaluate to true
or false.
Bug 34849

aarch64/CombineOp.v
@@ -67,6 +67,25 @@ Function combine_cond (cond: condition) (args: list valnum) : option(condition *
   | _, _ => None
   end.
 
+Definition combine_comparison (c: comparison) (x y: valnum) : option bool :=
+  match c with
+  | Ceq => if eq_valnum x y then Some true else None
+  | Cle => if eq_valnum x y then Some true else None
+  | Cge => if eq_valnum x y then Some true else None
+  | Cne => if eq_valnum x y then Some false else None
+  | Clt => if eq_valnum x y then Some false else None
+  | Cgt => if eq_valnum x y then Some false else None
+  end.
+
+Definition combine_cond' (cond: condition) (args: list valnum) : option bool :=
+  match cond, args with
+  | Ccomp c, x :: y :: nil => combine_comparison c x y
+  | Ccompu c, x :: y :: nil => combine_comparison c x y
+  | Ccompl c, x :: y :: nil => combine_comparison c x y
+  | Ccomplu c, x :: y :: nil => combine_comparison c x y
+  | _, _ => None
+  end.
+
 Function combine_addr (addr: addressing) (args: list valnum) : option(addressing * list valnum) :=
   match addr, args with
   | Aindexed n, x::nil =>
